{
 "cells": [
  {
   "cell_type": "markdown",
   "id": "92dd4a53",
   "metadata": {
    "vscode": {
     "languageId": "plaintext"
    }
   },
   "source": [
    "# Dot Product\n",
    "\n",
    "Given vectors $\\vec{x} = \\begin{bmatrix}x_1 \\\\ x_2 \\\\ \\dots \\\\ x_n\\end{bmatrix}$ and $\\vec{y} = \\begin{bmatrix}y_1 \\\\ y_2 \\\\ \\dots \\\\ y_n\\end{bmatrix}$ in $R^n$ the dot product is defined as :\n",
    "\n",
    "$\\vec{x} \\cdot \\vec{y} = x_1y_1 + x_2y_2 + \\dots + x_ny_n$\n",
    "\n",
    "It's easy to see the following properties based on the expansion and real number properties:\n",
    "\n",
    "a) commutative\n",
    "\n",
    "b) distributive over addition\n",
    "\n",
    "c) $(c\\vec{x}) \\cdot \\vec{y} = c(\\vec{x} \\cdot \\vec{y})$\n",
    "\n",
    "d) $\\vec{x} \\cdot \\vec{x} = \\Vert x \\Vert^2$ and $\\vec{x} \\cdot \\vec{x} = 0 \\iff \\vec{x} = \\vec{0}$\n",
    "\n",
    "**Proof of (d)**:\n",
    "\n",
    "Given $\\vec{x} = \\begin{bmatrix}x_1 \\\\ x_2 \\\\ \\dots \\\\ x_n\\end{bmatrix}$, \n",
    "\n",
    "$\\vec{x} \\cdot \\vec{x} = \\Vert x \\Vert^2 = x_1^2 + x_2^2 + \\dots + x_n^2 >= 0$\n",
    "\n",
    "If $\\vec{x} = \\vec{0}$ then $\\Vert x \\Vert^2 = 0$ => $\\vec{x} \\cdot \\vec{x}  = 0$\n",
    "Other way, if $\\vec{x} \\cdot \\vec{x} = \\Vert x \\Vert^2 = x_1^2 + x_2^2 + \\dots + x_n^2 = 0$, then $x_1, x_2, \\dots, x_n = 0$ ie. $\\vec{x} = \\vec{0}$\n",
    "\n",
    "\n",
    "## Corollary: $\\Vert \\vec{x} + \\vec{y} \\Vert^2 = \\Vert \\vec{x} \\Vert^2 + \\Vert \\vec{y} \\Vert^2 + 2 \\vec{x}.\\vec{y}$\n",
    "\n",
    "Proof:\n",
    "\n",
    "We use the commutative, distributive properties below.\n",
    "\n",
    "$\n",
    "\\begin{align}\n",
    "\\Vert \\vec{x} + \\vec{y} \\Vert^2 \n",
    "    &= (\\vec{x} + \\vec{y}) \\cdot (\\vec{x} + \\vec{y}) \\\\\n",
    "    &= (\\vec{x} \\cdot \\vec{x}) + (\\vec{y} \\cdot \\vec{y}) + 2 (\\vec{x} \\cdot \\vec{y}) \\\\\n",
    "    &= \\Vert \\vec{x} \\Vert^2 + \\Vert \\vec{y} \\Vert^2 + 2 (\\vec{x} \\cdot \\vec{y})\n",
    "\\end{align}\n",
    "$\n",
    "\n",
    "## Definition: Two vectors $\\vec{x}$ and $\\vec{y}$ are said to be orthogonal if $\\vec{x} \\cdot \\vec{y} = 0$\n",
    "\n",
    "Assume $\\vec{y} \\ne \\vec{0}$\n",
    "\n",
    "Given vectors $\\vec{x}$ and $\\vec{y}$, we can decompose x into 2 components parallel and perpendicular to y.\n",
    "\n",
    "\n",
    "$$proj_{y}\\vec{x} = x^{||} = \\frac{\\vec{x} \\cdot \\vec{y}}{\\Vert \\vec{y} \\Vert^2}\\vec{y}$$\n",
    "\n",
    "Note the parallel component is **independent** of the magnitude of y. If $\\hat{y} = \\frac{\\vec{y}}{\\Vert \\vec{y} \\Vert}$ is the unit vector in the direction of y, then\n",
    "\n",
    "$$proj_{y}\\vec{x} = (\\vec{x} \\cdot \\hat{y})\\hat{y}$$\n",
    "It follows that the perpendicular component:\n",
    "\n",
    "$$x^{\\perp} = \\vec{x} - \\frac{\\vec{x} \\cdot \\vec{y}}{\\Vert \\vec{y} \\Vert^2}\\vec{y}$$\n",
    "\n",
    "We can confirm the following:\n",
    "\n",
    "$\n",
    "\\begin{align}\n",
    "x^{\\perp} \\cdot \\vec{y} &= \\vec{x} \\cdot \\vec{y} - \\frac{\\vec{x} \\cdot \\vec{y}}{\\Vert \\vec{y} \\Vert^2}(\\vec{y} \\cdot \\vec{y}) \\\\\n",
    "                        &= \\vec{x} \\cdot \\vec{y} - \\vec{x} \\cdot \\vec{y} \\\\\n",
    "                        &= 0\n",
    "\\end{align}\n",
    "$\n",
    "\n",
    "\n",
    "Also, $x^{\\perp} + x^{||} = \\vec{x}$\n",
    "\n",
    "Note that $x^{||}$ is the unique multiple of y that satisfies:\n",
    "\n",
    "$(\\vec{x} - x^{||}) \\cdot \\vec{y} = 0$\n",
    "\n",
    "This is easy to see by expanding $(\\vec{x} - c\\vec{y}) \\cdot \\vec{y} = 0$\n",
    "\n",
    "Note that if $\\theta$ is the angle between $\\vec{x}$ and $\\vec{y}$, \n",
    "\n",
    "$\n",
    "\\begin{align}\n",
    "\\cos{\\theta} &= \\frac{\\text{signed length of proj of x}}{\\text{length of x}} \\\\\n",
    "             &= \\frac{\\vec{x} \\cdot \\vec{y}*(\\Vert \\vec{y} \\Vert)}{(\\Vert \\vec{y} \\Vert^2)(\\Vert \\vec{x} \\Vert)} \\\\\n",
    "             &= \\frac{\\vec{x} \\cdot \\vec{y}}{\\Vert \\vec{x} \\Vert \\Vert \\vec{y} \\Vert}\n",
    "\\end{align}\n",
    "$"
   ]
  },
  {
   "cell_type": "markdown",
   "id": "ecab090b",
   "metadata": {},
   "source": [
    "# Cauchy-Schwarz Inequality : $\\vec{x} \\cdot \\vec{y} \\le \\Vert \\vec{x} \\Vert \\Vert \\vec{y} \\Vert$\n",
    "\n",
    "The Cauchy-Schwarz Inequality:\n",
    "\n",
    "$$\\vec{x} \\cdot \\vec{y} \\le \\Vert \\vec{x} \\Vert \\Vert \\vec{y} \\Vert$$\n",
    "\n",
    "**Proof-1**:\n",
    "\n",
    "Let $\\vec{a} = \\begin{bmatrix}a_1 \\\\ a_2 \\\\ \\dots \\\\ a_n\\end{bmatrix}$ and $\\vec{n} = \\begin{bmatrix}b_1 \\\\ b_2 \\\\ \\dots \\\\ b_n\\end{bmatrix}$\n",
    "\n",
    "\n",
    "It follows that $\\vec{a} \\cdot \\vec{b} = \\sum_{i=1}^n a_ib_i$, $\\Vert \\vec{a} \\Vert^2 = \\sum_{i=1}^n a_i^2$, $\\Vert \\vec{b} \\Vert^2 = \\sum_{i=1}^n b_i^2$\n",
    "\n",
    "We start with the following expansion, where :\n",
    "\n",
    "$$\\sum_{i=1}^n (a_ix + b_i)^2 = x^2\\sum_{i=1}^n a_i^2 + 2x\\sum_{i=1}^n a_ib_i + \\sum_{i=1}^n b_i^2$$\n",
    "\n",
    "Because L.H.S. is the sum of squares, the sum is at the most zero (when $b_i = -xa_i$ for every i) - this would imply that the corresponding b_i and a_i are proportional (this will translate to the case where the two vectors are parallel).\n",
    "\n",
    "Leaving aside this case, we have all the roots being imaginary since the sum is always positive, which would imply the term for the root of the quadratic under the square root ($b^2 - 4ac$) is negative. Hence we get :\n",
    "\n",
    "\n",
    "$$ (2\\sum_{i=1}^n a_ib_i)^2 - 4 \\sum_{i=1}^n a_i^2 \\sum_{i=1}^n b_i^2 <= 0$$\n",
    "\n",
    "This implies:\n",
    "\n",
    "$$ \n",
    "\\begin{align}\n",
    "\\sum_{i=1}^n a_ib_i)^2 &<= \\sum_{i=1}^n a_i^2 \\sum_{i=1}^n b_i^2 \\\\\n",
    "(\\vec{a} \\cdot \\vec{b})^2 &<= \\Vert \\vec{a} \\Vert^2 \\Vert \\vec{b} \\Vert^2 \\\\\n",
    "\\text{Hence, } \\\\ \n",
    "\\vec{a} \\cdot \\vec{b} &<= \\Vert \\vec{a} \\Vert \\Vert \\vec{b} \\Vert\n",
    "                   \n",
    "\\end{align}\n",
    "$$\n",
    "\n",
    "As discussed earlier, equality is achieved when $b_i = -xa_i$ i.e. $\\vec{a} = c\\vec{b}$\n",
    "\n",
    "**Proof-2**:\n",
    "\n",
    "If $\\vec{y} = \\vec{0}$, there is nothing to prove.  If y is nonzero, let:\n",
    "\n",
    "$$\n",
    "\\begin{align}\n",
    "g(t) &= \\Vert \\vec{x} + t\\vec{y} \\Vert^2 \\\\\n",
    "     &= \\Vert \\vec{x} \\Vert^2 + 2t\\vec{x} \\cdot \\vec{y} + t^2\\Vert \\vec{y} \\Vert^2\n",
    "\\end{align}\n",
    "$$\n",
    "\n",
    "Since L.H.S. is always positive, and coefficient of $t^2$ is positive, the parabola has a non-negative minimum at $t_0 = -b/2a = -\\frac{\\vec{x} \\cdot \\vec{y}}{\\Vert \\vec{y} \\Vert^2}$\n",
    "\n",
    "i.e.\n",
    "\n",
    "$$\n",
    "\\begin{align}\n",
    "g(t_0) = \\Vert \\vec{x} \\Vert^2 - 2\\frac{(\\vec{x} \\cdot \\vec{y})^2}{\\Vert \\vec{y} \\Vert^2} + \\frac{(\\vec{x} \\cdot \\vec{y})^2}{\\Vert \\vec{y} \\Vert^2} &>= 0 \\\\\n",
    "\\text{Thus, } \\Vert \\vec{x} \\Vert^2 - \\frac{(\\vec{x} \\cdot \\vec{y})^2}{\\Vert \\vec{y} \\Vert^2} &>= 0  \\\\\n",
    "\\text{Or, } (\\vec{x} \\cdot \\vec{y})^2 &<= \\Vert \\vec{x} \\Vert^2 \\Vert \\vec{y} \\Vert^2\n",
    "\n",
    "\\end{align}\n",
    "$$\n",
    "\n",
    "## Corollary: When $t_0$ is minimum, $t_0\\vec{y} = -proj_y \\vec{x}$\n",
    "\n",
    "$t_0\\vec{y} = -\\frac{\\vec{x} \\cdot \\vec{y}}{\\Vert \\vec{y} \\Vert^2} \\vec{y} = -proj_y \\vec{x}$\n",
    "\n",
    "Hence,\n",
    "$x^{\\perp} = \\vec{x} -proj_y \\vec{x} = \\vec{x} + t_0\\vec{y} = g(t_0)$\n",
    "\n",
    "Note that : $\\vec{x} -proj_y \\vec{x}$ represents a vector drawn from  proj_y \\vec{x} (along $\\vec{y}$) to $\\vec{x}$ - and this is the shortest distance from anywhere along the line $t\\vec{y}$. And this shortest distance is the perpendicular from $\\vec{x}$ to the line $t\\vec{y}$.\n",
    "\n",
    "## Proof-3 : Ex 19: Using $\\Vert bx - ay \\Vert^2 >= 0$ where $a = \\Vert x \\Vert$, $b = \\Vert y \\Vert$\n",
    "\n",
    "$$\n",
    "\\begin{align}\n",
    "\\Vert b\\vec{x} - a\\vec{y} \\Vert^2 &>= 0 \\\\\n",
    "(b\\vec{x} - a\\vec{y}) \\cdot (b\\vec{x} - a\\vec{y}) &>= 0 \\\\\n",
    "2a^2b^2 - 2ab(\\vec{x} \\cdot \\vec{y}) &>= 0 \\\\\n",
    "\\vec{x} \\cdot \\vec{y} &<= ab = \\Vert x \\Vert \\Vert y \\Vert\n",
    "\n",
    "\n",
    "\\end{align}\n",
    "$$\n",
    "\n",
    "Equality holds when $\\Vert b\\vec{x} - a\\vec{y} \\Vert^2 = 0$ when means $\\vec{x} = (a/b)\\vec{y}$ i.e. x and y are parallel.\n"
   ]
  },
  {
   "cell_type": "markdown",
   "id": "afb32dce",
   "metadata": {},
   "source": [
    "# Triangle Inequality: \n",
    "\n",
    "$\\Vert \\vec{x} + \\vec{y} \\Vert \\le \\Vert \\vec{x} \\Vert + \\Vert \\vec{y} \\Vert$ \n",
    "\n",
    "Proof:\n",
    "\n",
    "$$\n",
    "\\begin{align}\n",
    "\\Vert \\vec{x} + \\vec{y} \\Vert^2 &=  (\\vec{x} + \\vec{y}) \\cdot  (\\vec{x} + \\vec{y}) \\\\\n",
    "        &= \\Vert \\vec{x} \\Vert^2 + \\Vert \\vec{y} \\Vert^2 + 2(\\vec{x} \\cdot \\vec{y})\n",
    "        &<= \\Vert \\vec{x} \\Vert^2 + \\Vert \\vec{y} \\Vert^2 + 2\\Vert \\vec{x} \\Vert \\Vert \\vec{y} \\Vert) \\text{ (applying Cauchy-Schwarz)} \\\\\n",
    "        &= (\\Vert \\vec{x} \\Vert + \\Vert \\vec{y} \\Vert)^2\n",
    "\n",
    "\\end{align}\n",
    "$$\n",
    "\n",
    "## Corollary (Ex 17): $\\Vert \\vec{x} - \\vec{y} \\Vert \\ge \\Vert \\vec{x} \\Vert - \\Vert \\vec{y} \\Vert$ \n",
    "\n",
    "Proof: || y + (x - y) || <= || y || + || x - y ||\n",
    "\n",
    "Hence || x - y || >= || x || - || y ||\n",
    "\n"
   ]
  },
  {
   "cell_type": "code",
   "execution_count": 2,
   "id": "49b82a7d",
   "metadata": {},
   "outputs": [
    {
     "data": {
      "text/latex": [
       "$\\displaystyle \\left[\\begin{matrix}-1\\\\0\\\\1\\end{matrix}\\right]$"
      ],
      "text/plain": [
       "Matrix([\n",
       "[-1],\n",
       "[ 0],\n",
       "[ 1]])"
      ]
     },
     "metadata": {},
     "output_type": "display_data"
    },
    {
     "data": {
      "text/latex": [
       "$\\displaystyle \\left[\\begin{matrix}4\\\\-4\\\\4\\end{matrix}\\right]$"
      ],
      "text/plain": [
       "Matrix([\n",
       "[ 4],\n",
       "[-4],\n",
       "[ 4]])"
      ]
     },
     "metadata": {},
     "output_type": "display_data"
    },
    {
     "data": {
      "text/latex": [
       "$\\displaystyle \\left[\\begin{matrix}-1\\\\0\\\\1\\end{matrix}\\right]$"
      ],
      "text/plain": [
       "Matrix([\n",
       "[-1],\n",
       "[ 0],\n",
       "[ 1]])"
      ]
     },
     "metadata": {},
     "output_type": "display_data"
    }
   ],
   "source": [
    "# Exercise 1.1-1 \n",
    "\n",
    "import sympy as s\n",
    "\n",
    "def proj(x,y):\n",
    "    return ((x.dot(y) / y.dot(y))*y)\n",
    "\n",
    "x = s.Matrix([3,-4,5])\n",
    "y = s.Matrix([-1,0,1])\n",
    "\n",
    "projx = proj(x,y)\n",
    "\n",
    "display(projx, x - projx)\n",
    "\n",
    "yhat = y / y.norm()\n",
    "\n",
    "display(x.dot(yhat)*yhat)"
   ]
  },
  {
   "cell_type": "markdown",
   "id": "e8158dc6",
   "metadata": {},
   "source": [
    "# Ex 6\n",
    "\n",
    "Given x + y + z = 0, what are the angles between the three vectors?\n",
    "\n",
    "x + y = -z\n",
    "\n",
    "x.z + y.z = -z.z = -1\n",
    "\n",
    "$\\cos{xz} + \\cos{yz} = -1$\n",
    "\n",
    "By symmetry, $\\cos{xz} = -1/2$ i.e. angle xz = 120 degrees. \n",
    "\n",
    "Geometrically, the three vectors for an equilateral triangle, with the origin as the centroid (since 1/3(x + y + z) = 0).\n",
    "\n"
   ]
  },
  {
   "cell_type": "markdown",
   "id": "ac622304",
   "metadata": {},
   "source": [
    "# Ex 7: Sum of Square of angles with basis vectors\n",
    "\n",
    "Let $\\theta_1, \\theta_2, \\theta_n$ be the angles made with basis vectors $e_1, e_2, e_n$ by a vector x.\n",
    "\n",
    "Then:\n",
    "\n",
    "$x \\cdot e_1 = x_i = \\Vert x \\Vert\\cos{\\theta_1}$\n",
    "\n",
    "Squaring and adding, we get :\n",
    "\n",
    "$\\Vert x \\Vert^2(\\cos^2{\\theta_1} + \\cos^2{\\theta_2} + \\dots + \\cos^2{\\theta_n}) = \\sum_i x_i^2 = \\Vert x \\Vert^2$.\n",
    "\n",
    "Thus,\n",
    "\n",
    "$\\cos^2{\\theta_1} + \\cos^2{\\theta_2} + \\dots + \\cos^2{\\theta_n} = 1$"
   ]
  },
  {
   "cell_type": "markdown",
   "id": "c84ba596",
   "metadata": {},
   "source": [
    "# Ex. 10 A parallelogram is a rectangle iff diagonals are of equal length\n",
    "\n",
    "Proof:\n",
    "\n",
    "Let vectors be u and v\n",
    "\n",
    "Diagonals are u - v, and u + v. \n",
    "\n",
    "|u-v| = |u + v| => (u - v).(u - v) = (u + v).(u + v) i.e. u.v = - u.v = 0. Thus u and v are perpendicular.\n",
    "\n",
    "If parallelogram is a rectangle, u.v = 0. Hence |u - v| = |u + v| ."
   ]
  },
  {
   "cell_type": "markdown",
   "id": "f2163b72",
   "metadata": {},
   "source": [
    "# Ex 12: Law of Cosines\n",
    "\n",
    "Prove: In triangle ABC, with opposite sides of length a, b, c and angle at C = $\\theta$\n",
    "\n",
    "$c^2 = a^2 + b^2 -2ab\\cos(\\theta)$\n",
    "\n",
    "Proof:\n",
    "\n",
    "|| AB ||^2 = || CB - CA ||^2 = (CB - CA) . (CB - CA) = CB.CB + CA.CA - 2CA.CB = a^2 + b^2 - 2ab Cos($\\theta$) "
   ]
  },
  {
   "cell_type": "markdown",
   "id": "756eff77",
   "metadata": {},
   "source": [
    "# Ex 13: Rhombus has diagonals perpendicular\n",
    "\n",
    "(u - v). (u + v) = 0 <=> ||u||^2 - ||v||^2 = 0 <=> ||u|| = ||v||\n",
    "\n"
   ]
  },
  {
   "cell_type": "markdown",
   "id": "0568c4f8",
   "metadata": {},
   "source": [
    "# Ex 14: triangle inscribed in circle with diameter as one of the sides is a right triangle.\n",
    "\n",
    "Let the origin be at the center of the circle.\n",
    "\n",
    "Let the ends of the diameter be $\\vec{a}$ and $-\\vec{a}$, with the point on the diameter being $\\vec{p}$.\n",
    "\n",
    "Then, || p || = || a || by definition of a circle.\n",
    "\n",
    "(a - p).(-a - p) = - (|| a ||^2 - || p ||^2) = 0\n",
    "\n",
    "Geometric Challenge: Locus of points transcribing a fixed angle $\\theta$ with two points a and b.\n",
    "\n",
    "Ans: See : https://jwilson.coe.uga.edu/emt725/AngleSubtendSegment/AngleSubtendSeg.html\n",
    "\n",
    "Summarizing: If we consider a point on the perpendicular bisector of ab, which subtends angle $2\\theta$, then we can see that the points form a circular arc around that point. We can consider another center on the opposite side also to get a second arc, except when the center lies on ab, in which case we get a perfect circle."
   ]
  },
  {
   "cell_type": "markdown",
   "id": "5b92e38a",
   "metadata": {},
   "source": [
    "# Ex 15(b): Given vectors $\\vec{y}$ and $\\vec{z}$, if $\\vec{x} \\cdot \\vec{y} = \\vec{x} \\cdot \\vec{z}$ for all $\\vec{x}$ in $R^n$, then $\\vec{y} = \\vec{z}$\n",
    "\n",
    "**Lemma: if $\\vec{x} \\cdot \\vec{y} = 0$ for all x in $R^n$, then $\\vec{x} = \\vec{0}$**\n",
    "\n",
    "Taking dot product with the basis vectors $e_1, e_2, e_n$, we can see all the coordinates are zero.\n",
    "\n",
    "Proof:\n",
    "\n",
    "x.y = x.z => x.(y-z) = 0 for all x in Rn => y-z = 0 => y = z."
   ]
  },
  {
   "cell_type": "markdown",
   "id": "fbfaf0bc",
   "metadata": {},
   "source": [
    "# Ex 16: a) Given $\\vec{x} = \\begin{bmatrix}x_1 \\\\ x_2 \\end{bmatrix}$, $\\rho(\\vec{x}) = \\begin{bmatrix}-x_2 \\\\ x_1 \\end{bmatrix}$ is orthogonal to $\\vec{x}$\n",
    "\n",
    "Proof: Just multiply by dot product\n",
    "\n",
    "**Interpret $\\vec{x} \\cdot \\rho(\\vec{y}) = -\\rho(\\vec{x}) \\cdot \\vec{y}$**\n",
    "\n",
    "One way to think is to show $\\rho(-x) = -\\rho(x)$, and $\\cos{\\theta} = -\\cos(\\pi - \\theta)$\n",
    "\n",
    "Let h,w,l are dimensions of cube. Note the long diagonal is || (h,w,l) || = c\n",
    "\n",
    "\n",
    "\n"
   ]
  },
  {
   "cell_type": "markdown",
   "id": "b1d9183e",
   "metadata": {},
   "source": [
    "# Ex 18: Max sum of sides of cube for given long diagonal of length c\n",
    "\n",
    "Sum of sides = h + w + l = (h,w,l).(1,1,1)\n",
    "\n",
    "c = ||(h,w,l)||\n",
    "\n",
    "(h,w,l).(1,1,1) <= ||(h,w,l)|| || (1,1,1) || = c $\\sqrt{3}$ (Cauchy-Schwarz)\n",
    "\n",
    "Equality is achieved when (h,w,l) = k(1,1,1) = (k,k,k). Then 3k = c $\\sqrt{3}$ or k = c/$\\sqrt{3}$\n",
    "\n",
    "\n",
    "\n"
   ]
  },
  {
   "cell_type": "markdown",
   "id": "03b89784",
   "metadata": {},
   "source": [
    "# Ex 20: Angle bisectors\n",
    "\n",
    "**Prove x + y bisects angle between x and , when || x || = || y ||**\n",
    "\n",
    "Cos(ang bet x and x + y) = x.(x + y) / ||x|| || x + y|| = ||x||^2 + x.y / || x || || x + y || \n",
    "                        = ||y||^2 + x.y / || y || || x + y || = cos (angle between y and x + y)\n",
    "\n",
    "**Prove bx + ay bisects angle x and y, where a = || x ||, b = || y ||**\n",
    "\n",
    "|| bx || = || y || || x || = || ay ||. Now apply previous result.\n"
   ]
  },
  {
   "cell_type": "markdown",
   "id": "059b2627",
   "metadata": {},
   "source": [
    "# Ex 22-26: Properties of triangle\n",
    "\n",
    "**AD is angle bisector of $\\angle{A}$, with D on BC. Prove ||BD||/||CD|| = ||AB|| / ||AC||**\n",
    "\n",
    "Proof: Let x = AB, y = AC, a = || x ||, b = || y ||\n",
    "\n",
    "then d lies on bx + ay i.e. AD = k(bx + ay)\n",
    "\n",
    "At the same time AD = y + s(x - y)\n",
    "kbx + kay = (1-s)y + sx\n",
    "\n",
    "kb = s or k = s/b\n",
    "ka = 1-s \n",
    "sa/b = 1-s => s(a + b)/b = 1 i.e. s = b/(a + b) => ||CD|| / || CB || = b / (a + b).\n",
    "||BD||/||CB|| = a/(a + b) and ||BD||/||CD|| = a/b.\n",
    "\n",
    "\n",
    "**Ex 23: Angle bisectors have a common point**\n",
    "\n",
    "Using the fact that s(bx + ay) = x + t(c(-x) + a(y-x) ), we get s = t, and sb = 1 - ct -at i.e. s = 1/a+b+c\n",
    "\n",
    "Thus the angle bisectors = 1/(a+b+c)(bx + ay)\n",
    "\n",
    "**Ex 24: Altitudes have a common point (orthocenter)**\n",
    "\n",
    "Let Q be the common point.\n",
    "\n",
    "Then $q = y + c\\rho(x) = x + d\\rho(y)$\n",
    "\n",
    "Taking dot product with y, we get:\n",
    "\n",
    "$y.y + c\\rho(x).y = x.y => c = (x.y - y.y)/\\rho(x).y$\n",
    "\n",
    "hence: \n",
    "\n",
    "$\\vec{q} = \\vec{y} + \\frac{\\vec{x} \\cdot \\vec{y} - \\Vert y \\Vert^2}{\\rho(x).y} \\rho(x)$\n",
    "\n",
    "Now q.(x - y) = y.x - || y ||^2 - (x.y - || y ||^2) = 0\n",
    "\n",
    "**Ex 25: Perpendicular bisectors intersect (circumcenter)**\n",
    "\n",
    "\n",
    "Let R be the common point. Then r = 1/2x + c $\\rho(x)$.\n",
    "\n",
    "But (y/2 - r).y = 0 (since z is the intersection of perp bisectors).\n",
    "\n",
    "1/2 (y.y) - r.y = 0\n",
    "\n",
    "\n",
    "1/2 y.y - (1/2x + c $\\rho(x)).y = 0\n",
    "1/2 || y ||^2 - 1/2 x.y -c $\\rho(x)$.y = 0\n",
    "\n",
    "c = 1/2 (|| y ||^2 - x.y)/($\\rho(x)$.y)\n",
    "\n",
    "Hence, \n",
    "\n",
    "$\\vec{r} = \\frac{1}{2}\\vec{x} + \\frac{1}{2} \\frac{\\Vert \\vec{y} \\Vert^2 - \\vec{x} \\cdot \\vec{y}}{\\rho(\\vec{x}) \\cdot \\vec{y}} \\rho(\\vec{x})$\n",
    "\n",
    "\n",
    "**Ex 26: Prove median, orthocenter and circumcenter are collinear**\n",
    "\n",
    "\n",
    "We have the median p, orthocenter q and circumcenter r as follows:\n",
    "\n",
    "$\\vec{p} = \\frac{1}{3} (\\vec{x} + \\vec{y})$\n",
    "\n",
    "$\\vec{q} = \\vec{y} + \\frac{\\vec{x} \\cdot \\vec{y} - \\Vert y \\Vert^2}{\\rho(x).y} \\rho(\\vec{x})$\n",
    "\n",
    "$\\vec{r} = \\frac{1}{2}\\vec{x} + \\frac{1}{2} \\frac{\\Vert \\vec{y} \\Vert^2 - \\vec{x} \\cdot \\vec{y}}{\\rho(\\vec{x}) \\cdot \\vec{y}} \\rho(\\vec{x})$\n",
    "\n",
    "$\\vec{r} - \\vec{q} = \\frac{1}{2}\\vec{x} - \\vec{y} + \\frac{3}{2} c \\rho(\\vec{x})$\n",
    "\n",
    "$\\vec{p} - \\vec{q} = \\frac{1}{3} \\vec{x} - \\frac{2}{3}\\vec{y} + c \\rho(\\vec{x}) = \\frac{2}{3} (\\vec{r} - \\vec{q})$\n",
    "\n"
   ]
  },
  {
   "cell_type": "markdown",
   "id": "bcacc1dd",
   "metadata": {},
   "source": []
  }
 ],
 "metadata": {
  "kernelspec": {
   "display_name": ".venv",
   "language": "python",
   "name": "python3"
  },
  "language_info": {
   "codemirror_mode": {
    "name": "ipython",
    "version": 3
   },
   "file_extension": ".py",
   "mimetype": "text/x-python",
   "name": "python",
   "nbconvert_exporter": "python",
   "pygments_lexer": "ipython3",
   "version": "3.12.8"
  }
 },
 "nbformat": 4,
 "nbformat_minor": 5
}
